trying to refactor
Signed-off-by: Oliver Flatt <oflatt@gmail.com>

cedar-lean/Cedar/Thm/TPE/WellTyped.lean
@@ -28,7 +28,7 @@ open Cedar.Spec
 open Cedar.Validation
 open Cedar.TPE
 
-def PEWellTyped (env : TypeEnv)
+abbrev PEWellTyped (env : TypeEnv)
   (r₁ r₂ : Residual)
   (req : Request)
   (preq : PartialRequest)
@@ -38,10 +38,255 @@ def PEWellTyped (env : TypeEnv)
   Residual.WellTyped env r₁ →
   Residual.WellTyped env r₂
 
+
+theorem partial_eval_well_typed_app₂ :
+  Residual.WellTyped env (TPE.evaluate expr1 preq pes) →
+  Residual.WellTyped env (TPE.evaluate expr2 preq pes) →
+  PEWellTyped env (Residual.binaryApp op expr1 expr2 ty) (TPE.apply₂ op (TPE.evaluate expr1 preq pes) (TPE.evaluate expr2 preq pes) pes ty) req preq es := by
+  unfold PEWellTyped
+  intros ih₁ ih₂ h_wf h_ref h_wt
+  unfold TPE.apply₂
+
+  split
+  . simp
+    split
+    . apply Residual.WellTyped.val
+      cases h_op
+      all_goals {
+        apply InstanceOfType.instance_of_bool
+        unfold InstanceOfBoolType
+        split <;> try simp
+        contradiction
+      }
+    repeat case _ =>
+      apply Residual.WellTyped.val
+      cases h_op
+      all_goals {
+        apply InstanceOfType.instance_of_bool
+        unfold InstanceOfBoolType
+        split <;> try simp
+        contradiction
+      }
+    . rename_i i j h₁ h₂
+      cases (i.add? j) <;> simp [someOrError]
+      . apply Residual.WellTyped.error
+      . apply Residual.WellTyped.val
+        cases h_op
+        all_goals {
+          apply InstanceOfType.instance_of_int
+        }
+    . rename_i i j h₁ h₂
+      cases (i.sub? j) <;> simp [someOrError]
+      . apply Residual.WellTyped.error
+      . apply Residual.WellTyped.val
+        cases h_op
+        all_goals {
+          apply InstanceOfType.instance_of_int
+        }
+    . rename_i i j h₁ h₂
+      cases (i.mul? j) <;> simp [someOrError]
+      . apply Residual.WellTyped.error
+      . apply Residual.WellTyped.val
+        cases h_op
+        all_goals {
+          apply InstanceOfType.instance_of_int
+        }
+    . rename_i i j h₁ h₂
+      apply Residual.WellTyped.val
+      cases h_op
+      all_goals {
+        apply InstanceOfType.instance_of_bool
+        simp [InstanceOfBoolType]
+      }
+    repeat case _ =>
+      apply Residual.WellTyped.val
+      cases h_op
+      all_goals {
+        apply InstanceOfType.instance_of_bool
+        simp [InstanceOfBoolType]
+      }
+    any_goals (
+      rename_i v1 v2 id1 id2 h₁ h₂
+      try cases (TPE.inₑ id1 id2 pes)
+      try cases (TPE.inₛ id1 id2 pes)
+      . simp [someOrSelf]
+        unfold TPE.apply₂.self
+        unfold Residual.asValue at h₁
+        unfold Residual.asValue at h₂
+        split at h₁
+        . split at h₂
+          . injection h₁
+            injection h₂
+            rename_i x v ty₁ h₃ h₄ h₅ ty₂ h₇ h₈ h₉
+            rw [h₃]
+            rw [h₇]
+            apply Residual.WellTyped.binaryApp
+            . apply Residual.WellTyped.val
+              subst expr1_eval
+              subst expr2_eval
+              rw [h₃] at h_expr1_wt
+              rw [h₇] at h_expr2_wt
+              cases h_expr1_wt
+              rename_i h₈
+              exact h₈
+            . apply Residual.WellTyped.val
+              subst expr1_eval
+              subst expr2_eval
+              rw [h₃] at h_expr1_wt
+              rw [h₇] at h_expr2_wt
+              cases h_expr2_wt
+              rename_i h₈
+              exact h₈
+            . rw [h₈]
+              rw [h₉]
+              cases h_op
+              . apply BinaryResidualWellTyped.memₑ
+                . simp [Residual.typeOf]
+                  rename_i ety₁ ety₂ eq₁ eq₂
+                  have hᵣ : (ty₁ = CedarType.entity ety₁) := by {
+                    subst expr1_eval
+                    subst expr2_eval
+                    have h₁₀ := tpe_evaluate_preserves_type h_wf h_ref_reconstructed h_expr1
+                    rw [← h₁₀] at eq₁
+                    rw [h₃] at eq₁
+                    simp [Residual.typeOf] at eq₁
+                    exact eq₁
+                  }
+                  exact hᵣ
+                . simp [Residual.typeOf]
+                  rename_i ety₁ ety₂ eq₁ eq₂
+                  have hᵣ : (ty₂ = CedarType.entity ety₂) := by {
+                    subst expr1_eval
+                    subst expr2_eval
+                    have h₁₀ := tpe_evaluate_preserves_type h_wf h_ref_reconstructed h_expr2
+                    rw [← h₁₀] at eq₂
+                    rw [h₇] at eq₂
+                    simp [Residual.typeOf] at eq₂
+                    exact eq₂
+                  }
+                  exact hᵣ
+              . apply BinaryResidualWellTyped.memₛ
+                . simp [Residual.typeOf]
+                  rename_i ety₁ ety₂ eq₁ eq₂
+                  have hᵣ : (ty₁ = CedarType.entity ety₁) := by {
+                    subst expr1_eval
+                    subst expr2_eval
+                    have h₁₀ := tpe_evaluate_preserves_type h_wf h_ref_reconstructed h_expr1
+                    rw [← h₁₀] at eq₁
+                    rw [h₃] at eq₁
+                    simp [Residual.typeOf] at eq₁
+                    exact eq₁
+                  }
+                  exact hᵣ
+                . simp [Residual.typeOf]
+                  rename_i ety₁ ety₂ eq₁ eq₂
+                  have hᵣ : (ty₂ = (CedarType.entity ety₂).set) := by {
+                    subst expr1_eval
+                    subst expr2_eval
+                    have h₁₀ := tpe_evaluate_preserves_type h_wf h_ref_reconstructed h_expr2
+                    rw [← h₁₀] at eq₂
+                    rw [h₇] at eq₂
+                    simp [Residual.typeOf] at eq₂
+                    exact eq₂
+                  }
+                  exact hᵣ
+          . contradiction
+        . contradiction
+      . simp [someOrSelf]
+        apply Residual.WellTyped.val
+        cases h_op
+        . apply InstanceOfType.instance_of_bool
+          simp [InstanceOfBoolType]
+        . apply InstanceOfType.instance_of_bool
+          simp [InstanceOfBoolType]
+    )
+    . rename_i v1 v2 id1 id2 h₁ h₂
+      cases TPE.hasTag id1 id2 pes
+      . simp [someOrSelf]
+        unfold TPE.apply₂.self
+        unfold Residual.asValue at h₁
+        unfold Residual.asValue at h₂
+        split at h₁
+        . split at h₂
+          . injection h₁
+            injection h₂
+            rename_i x v ty₁ h₃ h₄ h₅ ty₂ h₇ h₈ h₉
+            rw [h₃]
+            rw [h₇]
+            apply Residual.WellTyped.binaryApp
+            . apply Residual.WellTyped.val
+              subst expr1_eval
+              subst expr2_eval
+              rw [h₃] at h_expr1_wt
+              rw [h₇] at h_expr2_wt
+              cases h_expr1_wt
+              rename_i h₈
+              exact h₈
+            . apply Residual.WellTyped.val
+              subst expr1_eval
+              subst expr2_eval
+              rw [h₃] at h_expr1_wt
+              rw [h₇] at h_expr2_wt
+              cases h_expr2_wt
+              rename_i h₈
+              exact h₈
+            . rw [h₈]
+              rw [h₉]
+              cases h_op
+              . apply BinaryResidualWellTyped.hasTag
+                . simp [Residual.typeOf]
+                  rename_i ety₁ ety₂ eq₁ eq₂
+                  have hᵣ : (ty₁ = CedarType.entity ety₂) := by {
+                    subst expr1_eval
+                    subst expr2_eval
+                    have h₁₀ := tpe_evaluate_preserves_type h_wf h_ref_reconstructed h_expr1
+                    rw [← h₁₀] at eq₁
+                    rw [h₃] at eq₁
+                    simp [Residual.typeOf] at eq₁
+                    exact eq₁
+                  }
+                  exact hᵣ
+                . simp [Residual.typeOf]
+                  rename_i ety₁ ety₂ eq₁ eq₂
+                  have hᵣ : (ty₂ = CedarType.string) := by {
+                    subst expr1_eval
+                    subst expr2_eval
+                    have h₁₀ := tpe_evaluate_preserves_type h_wf h_ref_reconstructed h_expr2
+                    rw [← h₁₀] at eq₂
+                    rw [h₇] at eq₂
+                    simp [Residual.typeOf] at eq₂
+
+                    exact eq₂
+                  }
+                  exact hᵣ
+          . contradiction
+        . contradiction
+      . simp [someOrSelf]
+        apply Residual.WellTyped.val
+        cases h_op
+        . apply InstanceOfType.instance_of_bool
+          simp [InstanceOfBoolType]
+    . rename_i v1 v2 id1 id2 h₁ h₂
+      unfold TPE.getTag
+      split
+      . unfold someOrError
+        split
+        . apply Residual.WellTyped.val
+          rename Option (Data.Map Tag Value) => x
+          rename_i tags heq x₁ x₂ x₃ v h₃
+          cases h_op
+          rename_i ety ty h₄ h₅ h₆
+          sorry
+        . sorry
+      . sorry
+    repeat case _ => sorry
+  . sorry
+
+
 /--
 Helper theorem: Partial evaluation preserves well-typedness for variable residuals.
 -/
-theorem partial_evaluation_preserves_var_well_typedness      {env : TypeEnv}
+theorem partial_evaluation_well_typed_var      {env : TypeEnv}
   {v : Var}
   {ty : CedarType}
   {req : Request}
@@ -338,7 +583,7 @@ theorem partial_evaluation_preserves_residual_well_typedness
     -- Case: .var v ty
     -- Use the helper theorem for variable cases
     simp [TPE.evaluate]
-    exact partial_evaluation_preserves_var_well_typedness h_wf h_rref h_wt
+    exact partial_evaluation_well_typed_var h_wf h_rref h_wt
   | and a b ty =>
     -- Case: .and a b ty
     -- TPE.evaluate (.and a b ty) preq pes = TPE.and (TPE.evaluate a preq pes) (TPE.evaluate b preq pes) ty
@@ -517,159 +762,14 @@ theorem partial_evaluation_preserves_residual_well_typedness
               exact h_ty
   | binaryApp op expr1 expr2 ty =>
     simp [TPE.evaluate]
+    have h_wt₂ := h_wt
     cases h_wt with
     | binaryApp h_expr1 h_expr2 h_op =>
-      let expr1_eval := TPE.evaluate expr1 preq pes
-      let expr2_eval := TPE.evaluate expr2 preq pes
       have h_ref_reconstructed : RequestAndEntitiesRefine req es preq pes := ⟨h_rref, h_eref⟩
-      have h_expr1_wt : Residual.WellTyped env expr1_eval := partial_evaluation_preserves_residual_well_typedness h_wf h_ref_reconstructed h_expr1
-      have h_expr2_wt : Residual.WellTyped env expr2_eval := partial_evaluation_preserves_residual_well_typedness h_wf h_ref_reconstructed h_expr2
-      unfold TPE.apply₂
-      split
-      . simp
-        split
-        repeat case _ =>
-          apply Residual.WellTyped.val
-          cases h_op
-          all_goals {
-            apply InstanceOfType.instance_of_bool
-            unfold InstanceOfBoolType
-            split <;> try simp
-            contradiction
-          }
-        . rename_i i j h₁ h₂
-          cases (i.add? j) <;> simp [someOrError]
-          . apply Residual.WellTyped.error
-          . apply Residual.WellTyped.val
-            cases h_op
-            all_goals {
-              apply InstanceOfType.instance_of_int
-            }
-        . rename_i i j h₁ h₂
-          cases (i.sub? j) <;> simp [someOrError]
-          . apply Residual.WellTyped.error
-          . apply Residual.WellTyped.val
-            cases h_op
-            all_goals {
-              apply InstanceOfType.instance_of_int
-            }
-        . rename_i i j h₁ h₂
-          cases (i.mul? j) <;> simp [someOrError]
-          . apply Residual.WellTyped.error
-          . apply Residual.WellTyped.val
-            cases h_op
-            all_goals {
-              apply InstanceOfType.instance_of_int
-            }
-        . rename_i i j h₁ h₂
-          apply Residual.WellTyped.val
-          cases h_op
-          all_goals {
-            apply InstanceOfType.instance_of_bool
-            simp [InstanceOfBoolType]
-          }
-        repeat case _ =>
-          apply Residual.WellTyped.val
-          cases h_op
-          all_goals {
-            apply InstanceOfType.instance_of_bool
-            simp [InstanceOfBoolType]
-          }
-        . rename_i v1 v2 id1 id2 h₁ h₂
-          cases (TPE.inₑ id1 id2 pes)
-          . simp [someOrSelf]
-            unfold TPE.apply₂.self
-            unfold Residual.asValue at h₁
-            unfold Residual.asValue at h₂
-            split at h₁
-            . split at h₂
-              . injection h₁
-                injection h₂
-                rename_i x v ty₁ h₃ h₄ h₅ ty₂ h₇ h₈ h₉
-                rw [h₃]
-                rw [h₇]
-                apply Residual.WellTyped.binaryApp
-                . apply Residual.WellTyped.val
-                  subst expr1_eval
-                  subst expr2_eval
-                  rw [h₃] at h_expr1_wt
-                  rw [h₇] at h_expr2_wt
-                  cases h_expr1_wt
-                  rename_i h₈
-                  exact h₈
-                . apply Residual.WellTyped.val
-                  subst expr1_eval
-                  subst expr2_eval
-                  rw [h₃] at h_expr1_wt
-                  rw [h₇] at h_expr2_wt
-                  cases h_expr2_wt
-                  rename_i h₈
-                  exact h₈
-                . rw [h₈]
-                  rw [h₉]
-                  cases h_op
-                  . apply BinaryResidualWellTyped.memₑ
-                    . simp [Residual.typeOf]
-                      rename_i ety₁ ety₂ eq₁ eq₂
-                      have hᵣ : (ty₁ = CedarType.entity ety₁) := by {
-                        subst expr1_eval
-                        subst expr2_eval
-                        have h₁₀ := tpe_evaluate_preserves_type h_wf h_ref_reconstructed h_expr1
-                        rw [← h₁₀] at eq₁
-                        rw [h₃] at eq₁
-                        simp [Residual.typeOf] at eq₁
-                        exact eq₁
-                      }
-                      exact hᵣ
-                    . simp [Residual.typeOf]
-                      rename_i ety₁ ety₂ eq₁ eq₂
-                      have hᵣ : (ty₂ = CedarType.entity ety₂) := by {
-                        subst expr1_eval
-                        subst expr2_eval
-                        have h₁₀ := tpe_evaluate_preserves_type h_wf h_ref_reconstructed h_expr2
-                        rw [← h₁₀] at eq₂
-                        rw [h₇] at eq₂
-                        simp [Residual.typeOf] at eq₂
-                        exact eq₂
-                      }
-                      exact hᵣ
-                  . apply BinaryResidualWellTyped.memₛ
-                    . simp [Residual.typeOf]
-                      rename_i ety₁ ety₂ eq₁ eq₂
-                      have hᵣ : (ty₁ = CedarType.entity ety₁) := by {
-                        subst expr1_eval
-                        subst expr2_eval
-                        have h₁₀ := tpe_evaluate_preserves_type h_wf h_ref_reconstructed h_expr1
-                        rw [← h₁₀] at eq₁
-                        rw [h₃] at eq₁
-                        simp [Residual.typeOf] at eq₁
-                        exact eq₁
-                      }
-                      exact hᵣ
-                    . simp [Residual.typeOf]
-                      rename_i ety₁ ety₂ eq₁ eq₂
-                      have hᵣ : (ty₂ = (CedarType.entity ety₂).set) := by {
-                        subst expr1_eval
-                        subst expr2_eval
-                        have h₁₀ := tpe_evaluate_preserves_type h_wf h_ref_reconstructed h_expr2
-                        rw [← h₁₀] at eq₂
-                        rw [h₇] at eq₂
-                        simp [Residual.typeOf] at eq₂
-                        exact eq₂
-                      }
-                      exact hᵣ
-              . contradiction
-            . contradiction
-          . simp [someOrSelf]
-            apply Residual.WellTyped.val
-            cases h_op
-            . apply InstanceOfType.instance_of_bool
-              simp [InstanceOfBoolType]
-            . apply InstanceOfType.instance_of_bool
-              simp [InstanceOfBoolType]
-        . 
-        repeat case _ => sorry
-      . sorry
+      have h_expr1_wt : Residual.WellTyped env (TPE.evaluate expr1 preq pes) := partial_evaluation_preserves_residual_well_typedness h_wf h_ref_reconstructed h_expr1
+      have h_expr2_wt : Residual.WellTyped env (TPE.evaluate expr2 preq pes) := partial_evaluation_preserves_residual_well_typedness h_wf h_ref_reconstructed h_expr2
+
+      apply partial_eval_well_typed_app₂ h_expr1_wt h_expr2_wt h_wf h_rref h_wt₂
   | error ty =>
     simp [TPE.evaluate]
     exact h_wt
